Update the definitions of Array, Slice and Vec

backends/lean/Aeneas/Std/ArraySlice.lean
@@ -43,23 +43,23 @@ abbrev Array.length {α : Type u} {n : Usize} (v : Array α n) : Nat := v.val.le
 @[simp]
 abbrev Array.v {α : Type u} {n : Usize} (v : Array α n) : List α := v.val
 
-example {α: Type u} {n : Usize} (v : Array α n) : v.length ≤ Scalar.max ScalarTy.Usize := by
+example {α: Type u} {n : Usize} (v : Array α n) : v.length ≤ Usize.max := by
   scalar_tac
 
-def Array.make {α : Type u} (n : Usize) (init : List α) (hl : init.length = n.val := by rfl) :
+def Array.make {α : Type u} (n : Usize) (init : List α) (hl : init.length = n.val := by simp) :
   Array α n := ⟨ init, by apply hl ⟩
 
-example : Array Int (Usize.ofInt 2) := Array.make (Usize.ofInt 2) [0, 1]
+example : Array Int (Usize.ofNat 2) := Array.make (Usize.ofNat 2) [0, 1] (by simp)
 
-example : Array Int (Usize.ofInt 2) :=
+example : Array Int (Usize.ofNat 2) :=
   let x := 0
   let y := 1
-  Array.make (Usize.ofInt 2) [x, y]
+  Array.make (Usize.ofNat 2) [x, y]
 
-example : Result (Array Int (Usize.ofInt 2)) := do
+example : Result (Array Int (Usize.ofNat 2)) := do
   let x ← ok 0
   let y ← ok 1
-  ok (Array.make (Usize.ofInt 2) [x, y])
+  ok (Array.make (Usize.ofNat 2) [x, y])
 
 @[simp]
 abbrev Array.index_s {α : Type u} {n : Usize} [Inhabited α] (v : Array α n) (i : Nat) : α :=
@@ -70,17 +70,17 @@ abbrev Array.slice {α : Type u} {n : Usize} [Inhabited α] (v : Array α n) (i 
   v.val.slice i j
 
 def Array.index_usize {α : Type u} {n : Usize} (v: Array α n) (i: Usize) : Result α :=
-  match v.val.indexOpt i.toNat with
+  match v.val.indexOpt i.val with
   | none => fail .arrayOutOfBounds
   | some x => ok x
 
 -- For initialization
 def Array.repeat {α : Type u} (n : Usize) (x : α) : Array α n :=
-  ⟨ List.replicate n.toNat x, by have h := n.hmin; simp_all [Scalar.min] ⟩
+  ⟨ List.replicate n.val x, by simp_all ⟩
 
-@[pspec]
+@[progress]
 theorem Array.repeat_spec {α : Type u} (n : Usize) (x : α) :
-  ∃ a, Array.repeat n x = a ∧ a.val = List.replicate n.toNat x := by
+  ∃ a, Array.repeat n x = a ∧ a.val = List.replicate n.val x := by
   simp [Array.repeat]
 
 /- In the theorems below: we don't always need the `∃ ..`, but we use one
@@ -88,41 +88,41 @@ theorem Array.repeat_spec {α : Type u} (n : Usize) (x : α) :
    helps control the context.
  -/
 
-@[pspec]
+@[progress]
 theorem Array.index_usize_spec {α : Type u} {n : Usize} [Inhabited α] (v: Array α n) (i: Usize)
-  (hbound : i.toNat < v.length) :
-  ∃ x, v.index_usize i = ok x ∧ x = v.val.index i.toNat := by
+  (hbound : i.val < v.length) :
+  ∃ x, v.index_usize i = ok x ∧ x = v.val.index i.val := by
   simp only [index_usize]
   -- TODO: dependent rewrite
-  have h := List.indexOpt_eq_index v.val i.toNat (by scalar_tac)
+  have h := List.indexOpt_eq_index v.val i.val (by scalar_tac)
   simp [*]
 
 def Array.update_usize {α : Type u} {n : Usize} (v: Array α n) (i: Usize) (x: α) : Result (Array α n) :=
-  match v.val.indexOpt i.toNat with
+  match v.val.indexOpt i.val with
   | none => fail .arrayOutOfBounds
   | some _ =>
-    ok ⟨ v.val.update i.toNat x, by have := v.property; simp [*] ⟩
+    ok ⟨ v.val.update i.val x, by have := v.property; simp [*] ⟩
 
 def Array.update {α : Type u} {n : Usize} (v: Array α n) (i: Usize) (x: α) : Array α n :=
-  ⟨ v.val.update i.toNat x, by have := v.property; simp [*] ⟩
+  ⟨ v.val.update i.val x, by have := v.property; simp [*] ⟩
 
 @[simp]
 theorem Array.update_val_eq {α : Type u} {n : Usize} (v: Array α n) (i: Usize) (x: α) :
-  (v.update i x).val = v.val.update i.toNat x := by
+  (v.update i x).val = v.val.update i.val x := by
   simp [update]
 
 @[scalar_tac v.update i x]
 theorem Array.update_length {α : Type u} {n : Usize} (v: Array α n) (i: Usize) (x: α) :
   (v.update i x).length = v.length := by simp
 
-@[pspec]
+@[progress]
 theorem Array.update_usize_spec {α : Type u} {n : Usize} (v: Array α n) (i: Usize) (x : α)
-  (hbound : i.toNat < v.length) :
+  (hbound : i.val < v.length) :
   ∃ nv, v.update_usize i x = ok nv ∧
   nv = v.update i x
   := by
   simp only [update_usize]
-  have h := List.indexOpt_bounds v.val i.toNat
+  have h := List.indexOpt_bounds v.val i.val
   split
   . simp_all [length]
     scalar_tac
@@ -133,11 +133,11 @@ def Array.index_mut_usize {α : Type u} {n : Usize} (v: Array α n) (i: Usize) :
   let x ← index_usize v i
   ok (x, update v i)
 
-@[pspec]
+@[progress]
 theorem Array.index_mut_usize_spec {α : Type u} {n : Usize} [Inhabited α] (v: Array α n) (i: Usize)
-  (hbound : i.toNat < v.length) :
+  (hbound : i.val < v.length) :
   ∃ x, v.index_mut_usize i = ok (x, update v i) ∧
-  x = v.val.index i.toNat := by
+  x = v.val.index i.val := by
   simp only [index_mut_usize, Bind.bind, bind]
   have ⟨ x, h ⟩ := index_usize_spec v i hbound
   simp [h]
@@ -155,8 +155,8 @@ instance [BEq α] : BEq (Slice α) := SubtypeBEq _
 instance [BEq α] [LawfulBEq α] : LawfulBEq (Slice α) := SubtypeLawfulBEq _
 
 @[scalar_tac s]
-theorem Slice.length_ineq {α : Type u} (s : Slice α) : s.val.length ≤ Scalar.max ScalarTy.Usize := by
-  cases s; simp[Scalar.max, *]
+theorem Slice.length_ineq {α : Type u} (s : Slice α) : s.val.length ≤ Usize.max := by
+  cases s; simp[*]
 
 -- TODO: move/remove?
 @[scalar_tac s]
@@ -168,18 +168,18 @@ abbrev Slice.length {α : Type u} (v : Slice α) : Nat := v.val.length
 @[simp]
 abbrev Slice.v {α : Type u} (v : Slice α) : List α := v.val
 
-example {a: Type u} (v : Slice a) : v.length ≤ Scalar.max ScalarTy.Usize := by
+example {a: Type u} (v : Slice a) : v.length ≤ Usize.max := by
   scalar_tac
 
 def Slice.new (α : Type u) : Slice α := ⟨ [], by simp ⟩
 
 -- TODO: very annoying that the α is an explicit parameter
 abbrev Slice.len {α : Type u} (v : Slice α) : Usize :=
-  Usize.ofIntCore v.val.length (by constructor <;> scalar_tac)
+  Usize.ofNatCore v.val.length (by scalar_tac)
 
 @[simp]
 theorem Slice.len_val {α : Type u} (v : Slice α) : (Slice.len v).val = v.length :=
-  by rfl
+  by simp
 
 @[simp]
 abbrev Slice.index_s {α : Type u} [Inhabited α] (v: Slice α) (i: Nat) : α :=
@@ -190,7 +190,7 @@ abbrev Slice.slice {α : Type u} [Inhabited α] (s : Slice α) (i j : Nat) : Lis
   s.val.slice i j
 
 def Slice.index_usize {α : Type u} (v: Slice α) (i: Usize) : Result α :=
-  match v.val.indexOpt i.toNat with
+  match v.val.indexOpt i.val with
   | none => fail .arrayOutOfBounds
   | some x => ok x
 
@@ -199,41 +199,41 @@ def Slice.index_usize {α : Type u} (v: Slice α) (i: Usize) : Result α :=
    helps control the context.
  -/
 
-@[pspec]
+@[progress]
 theorem Slice.index_usize_spec {α : Type u} [Inhabited α] (v: Slice α) (i: Usize)
-  (hbound : i.toNat < v.length) :
-  ∃ x, v.index_usize i = ok x ∧ x = v.val.index i.toNat := by
+  (hbound : i.val < v.length) :
+  ∃ x, v.index_usize i = ok x ∧ x = v.val.index i.val := by
   simp only [index_usize]
   -- TODO: dependent rewrite
-  have h := List.indexOpt_eq_index v.val i.toNat (by scalar_tac)
+  have h := List.indexOpt_eq_index v.val i.val (by scalar_tac)
   simp [*]
 
 def Slice.update_usize {α : Type u} (v: Slice α) (i: Usize) (x: α) : Result (Slice α) :=
-  match v.val.indexOpt i.toNat with
+  match v.val.indexOpt i.val with
   | none => fail .arrayOutOfBounds
   | some _ =>
-    ok ⟨ v.val.update i.toNat x, by have := v.property; simp [*] ⟩
+    ok ⟨ v.val.update i.val x, by have := v.property; simp [*] ⟩
 
 def Slice.update {α : Type u} (v: Slice α) (i: Usize) (x: α) : Slice α :=
-  ⟨ v.val.update i.toNat x, by have := v.property; simp [*] ⟩
+  ⟨ v.val.update i.val x, by have := v.property; simp [*] ⟩
 
 @[simp]
 theorem Slice.update_val_eq {α : Type u} (v: Slice α) (i: Usize) (x: α) :
-  (v.update i x) = v.val.update i.toNat x := by
+  (v.update i x) = v.val.update i.val x := by
   simp [update]
 
 @[scalar_tac v.update i x]
 theorem Slice.update_length {α : Type u} (v: Slice α) (i: Usize) (x: α) :
   (v.update i x).length = v.length := by simp
 
-@[pspec]
+@[progress]
 theorem Slice.update_usize_spec {α : Type u} (v: Slice α) (i: Usize) (x : α)
-  (hbound : i.toNat < v.length) :
+  (hbound : i.val < v.length) :
   ∃ nv, v.update_usize i x = ok nv ∧
   nv = v.update i x
   := by
   simp only [update_usize]
-  have h := List.indexOpt_bounds v.val i.toNat
+  have h := List.indexOpt_bounds v.val i.val
   split
   . simp_all [length]; scalar_tac
   . simp [Slice.update]
@@ -243,11 +243,11 @@ def Slice.index_mut_usize {α : Type u} (v: Slice α) (i: Usize) :
   let x ← Slice.index_usize v i
   ok (x, Slice.update v i)
 
-@[pspec]
+@[progress]
 theorem Slice.index_mut_usize_spec {α : Type u} [Inhabited α] (v: Slice α) (i: Usize)
-  (hbound : i.toNat < v.length) :
+  (hbound : i.val < v.length) :
   ∃ x, v.index_mut_usize i = ok (x, Slice.update v i) ∧
-  x = v.val.index i.toNat := by
+  x = v.val.index i.val := by
   simp only [index_mut_usize, Bind.bind, bind]
   have ⟨ x, h ⟩ := Slice.index_usize_spec v i hbound
   simp [h]
@@ -261,7 +261,7 @@ theorem Slice.index_mut_usize_spec {α : Type u} [Inhabited α] (v: Slice α) (i
 def Array.to_slice {α : Type u} {n : Usize} (v : Array α n) : Result (Slice α) :=
   ok ⟨ v.val, by scalar_tac ⟩
 
-@[pspec]
+@[progress]
 theorem Array.to_slice_spec {α : Type u} {n : Usize} (v : Array α n) :
   ∃ s, to_slice v = ok s ∧ v.val = s.val := by simp [to_slice]
 
@@ -280,7 +280,7 @@ def Array.to_slice_mut {α : Type u} {n : Usize} (a : Array α n) :
   let s ← Array.to_slice a
   ok (s, Array.from_slice a)
 
-@[pspec]
+@[progress]
 theorem Array.to_slice_mut_spec {α : Type u} {n : Usize} (v : Array α n) :
   ∃ s, to_slice_mut v = ok (s, Array.from_slice v) ∧
   v.val = s.val
@@ -289,40 +289,40 @@ theorem Array.to_slice_mut_spec {α : Type u} {n : Usize} (v : Array α n) :
 def Array.subslice {α : Type u} {n : Usize} (a : Array α n) (r : Range Usize) : Result (Slice α) :=
   -- TODO: not completely sure here
   if r.start.val < r.end_.val ∧ r.end_.val ≤ a.val.length then
-    ok ⟨ a.val.slice r.start.toNat r.end_.toNat,
+    ok ⟨ a.val.slice r.start.val r.end_.val,
           by
-            have := a.val.slice_length_le r.start.toNat r.end_.toNat
+            have := a.val.slice_length_le r.start.val r.end_.val
             scalar_tac ⟩
   else
     fail panic
 
-@[pspec]
+@[progress]
 theorem Array.subslice_spec {α : Type u} {n : Usize} [Inhabited α] (a : Array α n) (r : Range Usize)
   (h0 : r.start.val < r.end_.val) (h1 : r.end_.val ≤ a.val.length) :
   ∃ s, subslice a r = ok s ∧
-  s.val = a.val.slice r.start.toNat r.end_.toNat ∧
-  (∀ i, 0 ≤ i → i + r.start.val < r.end_.val → s.val.index i.toNat = a.val.index (r.start.toNat + i.toNat))
+  s.val = a.val.slice r.start.val r.end_.val ∧
+  (∀ i, i + r.start.val < r.end_.val → s.val.index i = a.val.index (r.start.val + i))
   := by
-  simp [subslice, *]
-  intro i _ _
-  have := List.index_slice r.start.toNat r.end_.toNat i.toNat a.val (by scalar_tac) (by scalar_tac)
+  simp only [subslice, true_and, h0, h1, ↓reduceIte, ok.injEq, exists_eq_left', true_and]
+  intro i _
+  have := List.index_slice r.start.val r.end_.val i a.val (by scalar_tac) (by scalar_tac)
   simp [*]
 
 set_option maxHeartbeats 500000
 
 def Array.update_subslice {α : Type u} {n : Usize} (a : Array α n) (r : Range Usize) (s : Slice α) : Result (Array α n) :=
   -- TODO: not completely sure here
-  if h: r.start.toNat < r.end_.toNat ∧ r.end_.toNat ≤ a.length ∧ s.val.length = r.end_.toNat - r.start.toNat then
-    let s_beg := a.val.take r.start.toNat
-    let s_end := a.val.drop r.end_.toNat
-    have : s_beg.length = r.start.toNat := by
+  if h: r.start.val < r.end_.val ∧ r.end_.val ≤ a.length ∧ s.val.length = r.end_.val - r.start.val then
+    let s_beg := a.val.take r.start.val
+    let s_end := a.val.drop r.end_.val
+    have : s_beg.length = r.start.val := by
       scalar_tac
-    have : s_end.length = a.val.length - r.end_.toNat := by
+    have : s_end.length = a.val.length - r.end_.val := by
       scalar_tac
     let na := s_beg.append (s.val.append s_end)
     have : na.length = a.val.length:= by
       simp [na]; scalar_tac
-    ok ⟨ na, by simp_all; scalar_tac ⟩
+    ok ⟨ na, by simp_all ⟩
   else
     fail panic
 
@@ -331,15 +331,16 @@ def Array.update_subslice {α : Type u} {n : Usize} (a : Array α n) (r : Range 
 -- operations/
 -- We should introduce special symbols for the monadic arithmetic operations
 -- (the user will never write those symbols directly).
-@[pspec]
+@[progress]
 theorem Array.update_subslice_spec {α : Type u} {n : Usize} [Inhabited α] (a : Array α n) (r : Range Usize) (s : Slice α)
-  (_ : r.start.toNat < r.end_.toNat) (_ : r.end_.toNat ≤ a.length) (_ : s.length = r.end_.toNat - r.start.toNat) :
+  (_ : r.start.val < r.end_.val) (_ : r.end_.val ≤ a.length) (_ : s.length = r.end_.val - r.start.val) :
   ∃ na, update_subslice a r s = ok na ∧
-  (∀ i, 0 ≤ i → i < r.start.toNat → na.index_s i = a.index_s i) ∧
-  (∀ i, r.start.toNat ≤ i → i < r.end_.toNat → na.index_s i = s.index_s (i - r.start.toNat)) ∧
-  (∀ i, r.end_.toNat ≤ i → i < n.toNat → na.index_s i = a.index_s i) := by
-  simp [update_subslice, *]
-  have h := List.replace_slice_index r.start.toNat r.end_.toNat a.val s.val
+  (∀ i, i < r.start.val → na.index_s i = a.index_s i) ∧
+  (∀ i, r.start.val ≤ i → i < r.end_.val → na.index_s i = s.index_s (i - r.start.val)) ∧
+  (∀ i, r.end_.val ≤ i → i < n.val → na.index_s i = a.index_s i) := by
+  simp only [update_subslice, length, and_true, true_and, List.append_eq,
+    index_s, Slice.index_s, ↓reduceDIte, ok.injEq, exists_eq_left', *]
+  have h := List.replace_slice_index r.start.val r.end_.val a.val s.val
     (by scalar_tac) (by scalar_tac) (by scalar_tac)
   simp [List.replace_slice] at h
   have ⟨ h0, h1, h2 ⟩ := h
@@ -358,31 +359,31 @@ theorem Array.update_subslice_spec {α : Type u} {n : Usize} [Inhabited α] (a :
 def Slice.subslice {α : Type u} (s : Slice α) (r : Range Usize) : Result (Slice α) :=
   -- TODO: not completely sure here
   if r.start.val < r.end_.val ∧ r.end_.val ≤ s.length then
-    ok ⟨ s.val.slice r.start.toNat r.end_.toNat,
+    ok ⟨ s.val.slice r.start.val r.end_.val,
           by
-            have := s.val.slice_length_le r.start.toNat r.end_.toNat
+            have := s.val.slice_length_le r.start.val r.end_.val
             scalar_tac ⟩
   else
     fail panic
 
-@[pspec]
+@[progress]
 theorem Slice.subslice_spec {α : Type u} [Inhabited α] (s : Slice α) (r : Range Usize)
-  (h0 : r.start.toNat < r.end_.toNat) (h1 : r.end_.toNat ≤ s.val.length) :
+  (h0 : r.start.val < r.end_.val) (h1 : r.end_.val ≤ s.val.length) :
   ∃ ns, subslice s r = ok ns ∧
-  ns.val = s.slice r.start.toNat r.end_.toNat ∧
-  (∀ i, i + r.start.toNat < r.end_.toNat → ns.index_s i = s.index_s (r.start.toNat + i))
+  ns.val = s.slice r.start.val r.end_.val ∧
+  (∀ i, i + r.start.val < r.end_.val → ns.index_s i = s.index_s (r.start.val + i))
   := by
   simp_all [subslice]
   intro i _
-  have := List.index_slice r.start.toNat r.end_.toNat i s.val (by scalar_tac) (by scalar_tac)
+  have := List.index_slice r.start.val r.end_.val i s.val (by scalar_tac) (by scalar_tac)
   simp [*]
 
 def Slice.update_subslice {α : Type u} (s : Slice α) (r : Range Usize) (ss : Slice α) : Result (Slice α) :=
   -- TODO: not completely sure here
-  if h: r.start.toNat < r.end_.toNat ∧ r.end_.toNat ≤ s.length ∧ ss.val.length = r.end_.toNat - r.start.toNat then
-    let s_beg := s.val.take r.start.toNat
-    let s_end := s.val.drop r.end_.toNat
-    have : s_beg.length = r.start.toNat := by scalar_tac
+  if h: r.start.val < r.end_.val ∧ r.end_.val ≤ s.length ∧ ss.val.length = r.end_.val - r.start.val then
+    let s_beg := s.val.take r.start.val
+    let s_end := s.val.drop r.end_.val
+    have : s_beg.length = r.start.val := by scalar_tac
     have : s_end.length = s.val.length - r.end_.val := by scalar_tac
     let ns := s_beg.append (ss.val.append s_end)
     have : ns.length = s.val.length := by simp [ns, *]; scalar_tac
@@ -390,15 +391,15 @@ def Slice.update_subslice {α : Type u} (s : Slice α) (r : Range Usize) (ss : S
   else
     fail panic
 
-@[pspec]
+@[progress]
 theorem Slice.update_subslice_spec {α : Type u} [Inhabited α] (a : Slice α) (r : Range Usize) (ss : Slice α)
-  (_ : r.start.toNat < r.end_.toNat) (_ : r.end_.toNat ≤ a.length) (_ : ss.length = r.end_.toNat - r.start.toNat) :
+  (_ : r.start.val < r.end_.val) (_ : r.end_.val ≤ a.length) (_ : ss.length = r.end_.val - r.start.val) :
   ∃ na, update_subslice a r ss = ok na ∧
-  (∀ i, i < r.start.toNat → na.index_s i = a.index_s i) ∧
-  (∀ i, r.start.toNat ≤ i → i < r.end_.toNat → na.index_s i = ss.index_s (i - r.start.toNat)) ∧
-  (∀ i, r.end_.toNat ≤ i → i < a.length → na.index_s i = a.index_s i) := by
+  (∀ i, i < r.start.val → na.index_s i = a.index_s i) ∧
+  (∀ i, r.start.val ≤ i → i < r.end_.val → na.index_s i = ss.index_s (i - r.start.val)) ∧
+  (∀ i, r.end_.val ≤ i → i < a.length → na.index_s i = a.index_s i) := by
   simp [update_subslice, *]
-  have h := List.replace_slice_index r.start.toNat r.end_.toNat a.val ss.val
+  have h := List.replace_slice_index r.start.val r.end_.val a.val ss.val
     (by scalar_tac) (by scalar_tac) (by scalar_tac)
   simp [List.replace_slice, *] at h
   have ⟨ h0, h1, h2 ⟩ := h
@@ -416,12 +417,12 @@ theorem Slice.update_subslice_spec {α : Type u} [Inhabited α] (a : Slice α) (
 
 @[simp]
 theorem Array.update_index_eq α n [Inhabited α] (x : Array α n) (i : Usize) :
-  x.update i (x.val.index i.toNat) = x := by
+  x.update i (x.val.index i.val) = x := by
   simp [Array, Subtype.eq_iff]
 
 @[simp]
 theorem Slice.update_index_eq α [Inhabited α] (x : Slice α) (i : Usize) :
-  x.update i (x.val.index i.toNat) = x := by
+  x.update i (x.val.index i.val) = x := by
   simp [Slice, Subtype.eq_iff]
 
 /- Trait declaration: [core::slice::index::private_slice_index::Sealed] -/
