backends/lean/Aeneas/Std/Vec.lean
@@ -28,8 +28,8 @@ instance [BEq α] : BEq (Vec α) := SubtypeBEq _
 instance [BEq α] [LawfulBEq α] : LawfulBEq (Vec α) := SubtypeLawfulBEq _
 
 @[scalar_tac v]
-theorem Vec.len_ineq {α : Type u} (v : Vec α) : 0 ≤ v.val.length ∧ v.val.length ≤ Scalar.max ScalarTy.Usize := by
-  cases v; simp[Scalar.max, *]
+theorem Vec.len_ineq {α : Type u} (v : Vec α) : 0 ≤ v.val.length ∧ v.val.length ≤ Usize.max := by
+  cases v; simp[*]
 
 -- TODO: move/remove?
 @[scalar_tac v]
@@ -41,7 +41,7 @@ abbrev Vec.length {α : Type u} (v : Vec α) : Nat := v.val.length
 @[simp]
 abbrev Vec.v {α : Type u} (v : Vec α) : List α := v.val
 
-example {a: Type u} (v : Vec a) : v.length ≤ Scalar.max ScalarTy.Usize := by
+example {a: Type u} (v : Vec a) : v.length ≤ Usize.max := by
   scalar_tac
 
 abbrev Vec.new (α : Type u): Vec α := ⟨ [], by simp ⟩
@@ -52,26 +52,22 @@ instance (α : Type u) : Inhabited (Vec α) := by
 
 @[simp]
 abbrev Vec.len {α : Type u} (v : Vec α) : Usize :=
-  Usize.ofIntCore v.val.length (by constructor <;> scalar_tac)
+  Usize.ofNatCore v.val.length (by scalar_tac)
 
 @[simp]
 theorem Vec.len_val {α : Type u} (v : Vec α) : (Vec.len v).val = v.length :=
-  by rfl
+  by simp
 
 @[irreducible]
 def Vec.push {α : Type u} (v : Vec α) (x : α) : Result (Vec α)
   :=
   let nlen := List.length v.val + 1
   if h : nlen ≤ U32.max || nlen ≤ Usize.max then
-    have h : nlen ≤ Usize.max := by
-      simp [Usize.max] at *
-      have hm := Usize.refined_max.property
-      cases h <;> cases hm <;> simp [U32.max, U64.max] at * <;> try omega
-    ok ⟨ List.concat v.val x, by simp at *; assumption ⟩
+    ok ⟨ List.concat v.val x, by simp; scalar_tac ⟩
   else
     fail maximumSizeExceeded
 
-@[pspec]
+@[progress]
 theorem Vec.push_spec {α : Type u} (v : Vec α) (x : α) (h : v.val.length < Usize.max) :
   ∃ v1, v.push x = ok v1 ∧
   v1.val = v.val ++ [x] := by
@@ -81,52 +77,52 @@ theorem Vec.push_spec {α : Type u} (v : Vec α) (x : α) (h : v.val.length < Us
 
 def Vec.insert {α : Type u} (v: Vec α) (i: Usize) (x: α) : Result (Vec α) :=
   if i.val < v.length then
-    ok ⟨ v.val.update i.toNat x, by have := v.property; simp [*] ⟩
+    ok ⟨ v.val.update i x, by have := v.property; simp [*] ⟩
   else
     fail arrayOutOfBounds
 
-@[pspec]
+@[progress]
 theorem Vec.insert_spec {α : Type u} (v: Vec α) (i: Usize) (x: α)
   (hbound : i.val < v.length) :
-  ∃ nv, v.insert i x = ok nv ∧ nv.val = v.val.update i.toNat x := by
+  ∃ nv, v.insert i x = ok nv ∧ nv.val = v.val.update i x := by
   simp [insert, *]
 
 def Vec.index_usize {α : Type u} (v: Vec α) (i: Usize) : Result α :=
-  match v.val.indexOpt i.toNat with
+  match v.val.indexOpt i with
   | none => fail .arrayOutOfBounds
   | some x => ok x
 
-@[pspec]
+@[progress]
 theorem Vec.index_usize_spec {α : Type u} [Inhabited α] (v: Vec α) (i: Usize)
   (hbound : i.val < v.length) :
-  ∃ x, v.index_usize i = ok x ∧ x = v.val.index i.toNat := by
+  ∃ x, v.index_usize i = ok x ∧ x = v.val.index i := by
   simp only [index_usize]
   -- TODO: dependent rewrite
-  have h := List.indexOpt_eq_index v.val i.toNat (by scalar_tac)
+  have h := List.indexOpt_eq_index v.val i (by scalar_tac)
   simp [*]
 
 def Vec.update {α : Type u} (v: Vec α) (i: Usize) (x: α) : Vec α :=
-  ⟨ v.val.update i.toNat x, by have := v.property; simp [*] ⟩
+  ⟨ v.val.update i x, by have := v.property; simp [*] ⟩
 
 @[simp]
 theorem Vec.update_val_eq {α : Type u} (v: Vec α) (i: Usize) (x: α) :
-  (v.update i x).val = v.val.update i.toNat x := by
+  (v.update i x).val = v.val.update i x := by
   simp [update]
 
 def Vec.update_usize {α : Type u} (v: Vec α) (i: Usize) (x: α) : Result (Vec α) :=
-  match v.val.indexOpt i.toNat with
+  match v.val.indexOpt i with
   | none => fail .arrayOutOfBounds
   | some _ =>
-    ok ⟨ v.val.update i.toNat x, by have := v.property; simp [*] ⟩
+    ok ⟨ v.val.update i x, by have := v.property; simp [*] ⟩
 
-@[pspec]
+@[progress]
 theorem Vec.update_usize_spec {α : Type u} (v: Vec α) (i: Usize) (x : α)
   (hbound : i.val < v.length) :
   ∃ nv, v.update_usize i x = ok nv ∧
   nv = v.update i x
   := by
   simp only [update_usize]
-  have h := List.indexOpt_bounds v.val i.toNat
+  have h := List.indexOpt_bounds v.val i
   split
   . simp_all [length]; scalar_tac
   . simp [Vec.update]
@@ -143,11 +139,11 @@ def Vec.index_mut_usize {α : Type u} (v: Vec α) (i: Usize) :
   | fail e => fail e
   | div => div
 
-@[pspec]
+@[progress]
 theorem Vec.index_mut_usize_spec {α : Type u} [Inhabited α] (v: Vec α) (i: Usize)
   (hbound : i.val < v.length) :
   ∃ x, v.index_mut_usize i = ok (x, v.update i) ∧
-  x = v.val.index i.toNat
+  x = v.val.index i
   := by
   simp only [index_mut_usize]
   have ⟨ x, h ⟩ := index_usize_spec v i hbound
@@ -245,17 +241,17 @@ def core.ops.deref.DerefMutVec {T : Type} :
 def alloc.vec.Vec.resize {T : Type} (cloneInst : core.clone.Clone T)
   (v : alloc.vec.Vec T) (new_len : Usize) (value : T) : Result (alloc.vec.Vec T) := do
   if new_len.val < v.length then
-    ok ⟨ v.val.resize new_len.toNat value, by scalar_tac ⟩
+    ok ⟨ v.val.resize new_len value, by scalar_tac ⟩
   else
     let value ← cloneInst.clone value
-    ok ⟨ v.val.resize new_len.toNat value, by scalar_tac ⟩
+    ok ⟨ v.val.resize new_len value, by scalar_tac ⟩
 
-@[pspec]
+@[progress]
 theorem alloc.vec.Vec.resize_spec {T} (cloneInst : core.clone.Clone T)
   (v : alloc.vec.Vec T) (new_len : Usize) (value : T)
   (hClone : cloneInst.clone value = ok value) :
   ∃ nv, alloc.vec.Vec.resize cloneInst v new_len value = ok nv ∧
-    nv.val = v.val.resize new_len.toNat value := by
+    nv.val = v.val.resize new_len value := by
   rw [resize]
   split
   . simp
@@ -263,7 +259,7 @@ theorem alloc.vec.Vec.resize_spec {T} (cloneInst : core.clone.Clone T)
 
 @[simp]
 theorem alloc.vec.Vec.update_index_eq α [Inhabited α] (x : alloc.vec.Vec α) (i : Usize) :
-  x.update i (x.val.index i.toNat) = x := by
+  x.update i (x.val.index i) = x := by
   simp [Vec, Subtype.eq_iff]
 
 end Std
