backends/lean/Aeneas/ScalarTac/IntTac.lean
@@ -214,7 +214,9 @@ def intTac (tacName : String) (config : Config)
              ``not_false_eq_true, ``not_true_eq_false,
              ``true_and, ``and_true, ``false_and, ``and_false,
              ``true_or, ``or_true,``false_or, ``or_false,
-             ``Bool.true_eq_false, ``Bool.false_eq_true] [])
+             ``Bool.true_eq_false, ``Bool.false_eq_true,
+             -- The following lemmas are used to simplify occurrences of `decide`
+             ``decide_eq_true_eq, ``Bool.or_eq_true, ``Bool.and_eq_true,] [])
         allGoalsNoRecover (do
           trace[ScalarTac] "Goal after simplification: {← getMainGoal}"
           trace[ScalarTac] "Calling omega"
